ext gcd to positive

examples/modular_inversion/proofs/ext_gcd_optmized.ec
@@ -14,6 +14,17 @@ module OptExtGcd = {
       return (t2,t3);
   }
 
+  proc simplify_ts_pos(t2:int,t3: int,u:int,v:int) = {
+      while (even t3){
+        if (even t2){
+          (t2,t3) <- (t2 %/2, t3 %/2);
+        }else{
+          (t2,t3) <- ((t2+u) %/2, t3 %/2);
+        }
+      }
+      return (t2,t3);
+  }
+
   (* assumption: u odd *)
   proc main1(u : int, v : int) = {
     var u1,u2,u3,v1,v2,v3,t1,t2,t3;
@@ -151,10 +162,72 @@ module OptExtGcd = {
        }
       return (u2, u3);
   }  
-  
-  
-}.
 
+
+    proc main6(u : int, v : int) = {
+      var u2,u3,v2,v3,t2,t3;
+
+      (u2,u3) <- (0, u);
+      (v2,v3) <- (u-1, v);
+      (t2,t3) <- (1, v);
+
+      (t2,t3) <@ simplify_ts_pos(t2, v, u, v);
+      (v2, v3) <- (u-t2, t3);
+
+      (t2, t3) <- (u2-v2, `|u3-v3|);
+
+      while (t3 <> 0){
+        (t2,t3) <@ simplify_ts_pos(t2, t3, u, v);
+        if (v3 < u3){
+          (u2, u3) <- (t2, t3);
+        }else{
+          (v2, v3) <- (u-t2, t3);
+        }
+
+        t2 <- u2 - v2;
+        if (v3 < u3){
+          t3 <- u3 - v3;
+        }else{
+          t3 <- v3 - u3;
+        }
+
+       }
+      return (-u2, u3);
+  }    
+}.
+ 
+
+lemma opt_5_eq :
+     equiv [ OptExtGcd.simplify_ts ~ OptExtGcd.simplify_ts_pos :  odd u{1} /\
+      t2{1} = -t2{2} /\ ={t3,u,v} ==> res{1}.`1 = -res{2}.`1 /\ res{1}.`2 = res{2}.`2 ].
+proc. simplify.
+while ( t2{1} = -t2{2} /\ ={t3, u, v} /\ odd u{1}).
+wp. skip. progress. smt(@Int). smt(@Int). smt.
+have ->: (-t2{2}) - u{2} =  - ((t2{2}) + u{2}). smt(@Int).
+pose x := t2{2} + u{2}.
+rewrite dvdNdiv. auto.
+smt(@Int @IntDiv).
+smt.    
+skip. progress. qed.
+    
+   
+lemma opt_5 : equiv[ OptExtGcd.main5 ~ OptExtGcd.main6 : ={arg} /\ 0 < u{1} /\ 0 < v{1}
+  /\ odd u{1}    ==>  res{1}.`1 = res{2}.`1 /\ res{1}.`2 = res{2}.`2].
+proc.
+seq 3 3 : (={u,v,u3,v3,t3} /\ t2{1} = -t2{2} /\ u2{1} = -u2{2} /\ v2{1} = -v2{2} /\ 0 < u{1} /\ 0 < v{1} /\ t2{1} = -1 /\ u2{1} = 0 /\ v2{1} = 1 - u{2} /\ 0 <= v2{2} /\ odd u{1} ).
+wp. skip. progress. smt. smt.
+seq 1 1 : (={u,v,u3,v3,t3} /\ t2{1} = -t2{2} /\ u2{1} = -u2{2} /\ u2{2} = 0 /\ v2{1} = -v2{2} /\ 0 < u{1} /\ 0 < v{1} /\ odd u{1}  ).
+call opt_5_eq. simplify. skip. progress. smt(). 
+seq 1 1 : (={u,v,u3,v3,t3} /\ t2{1} = -t2{2} /\ u2{1} = -u2{2} /\ v2{1} = -v2{2} /\ 0 < u{1} /\ 0 < v{1}  /\ odd u{1}).
+wp. skip. progress.  simplify.  smt. 
+seq 1 1 : (={u,v,u3,v3,t3} /\ t2{1} = -t2{2} /\ u2{1} = -u2{2} /\ v2{1} = -v2{2} /\ 0 < u{1} /\ 0 < v{1} /\ odd u{1} ).      
+wp. skip. progress.  simplify. smt.
+while (={u,v,u3,v3,t3} /\ t2{1} = -t2{2} /\ u2{1} = -u2{2} /\ v2{1} = -v2{2} /\ 0 < u{1} /\ 0 < v{1} /\ odd u{1} ).
+seq 1 1 : ((={u,v,u3,v3,t3} /\ t2{1} = -t2{2} /\ u2{1} = -u2{2} /\ v2{1} = -v2{2} /\ 0 < u{1} /\ 0 < v{1} /\ odd u{1} )). call opt_5_eq. simplify. skip. progress. 
+wp. skip. progress. smt. smt. smt. smt. smt. smt. simplify.
+skip. progress.
+qed.     
+     
 
 lemma opt_0 : equiv[ ExtGCD.main2 ~ OptExtGcd.main1 : ={arg} /\ 0 < u{1} /\ 0 < v{1} ==> ={res} ].
 proc. sp. simplify.
